\documentclass[a4paper,12pt]{article}
\begin{document}
\noindent 1.
\begin{eqnarray*}
\frac{n!}{r!(n-r)!} & = & \frac{(n-1)!}{r!(n-1-r)!} + \frac{(n-1)!}{(r-1)!((n-1)-(r-1))!} \\
                    & = & \frac{(n-1)!}{r!(n-1-r)!} + \frac{(n-1)!}{(r-1)!(n-r)!} \\
                    & = & ... \\
                    & = & \frac{(n-r+r)(n-1)!}{r(r-1)!(n-r)(n-r-1)!} \\
                    & = & \frac{(n)(n-1)!}{r(r-1)!(n-r)(n-r-1)!} \\
                    & = & \frac{n!}{r!(n-r)!}
\end{eqnarray*}
\noindent 2.

\begin{center}
$ \varphi = \exists_x :\forall_y : y \in x$

$ \forall_x(x \neq \emptyset \rightarrow \exists_y \in x(y \bigcap x = \emptyset))$

$ \exists_x(x \neq \emptyset \rightarrow \forall_y \in x(y \bigcap x \neq \emptyset))$

$ \exists_y \in x(y \bigcap x \neq \emptyset)$

$ \{ y \bigcap x = \emptyset, y \bigcap x \neq \emptyset \} \vdash \phi$
\end{center}
\noindent 3.

\begin{center}
\[ T(n) = \left[ T\left(\frac{n}{2^i}\right) + \sum_{k=0}^{i-1} \left( \textrm{log}_2 \frac{n}{2^k} \right) \right] + 1 \]
\end{center}
\end{document}